Primitive_Matchers/IpAddresses_Normalize.thy
@@ -36,24 +36,6 @@ subsection{*Normalizing IP Addresses*}
   
 
 
-  fun l2br_negation_type_intersect :: "('a::len word \<times> 'a::len word) negation_type list \<Rightarrow> 'a::len wordinterval" where
-    "l2br_negation_type_intersect [] = wordinterval_UNIV" |
-    "l2br_negation_type_intersect ((Pos (s,e))#ls) = wordinterval_intersection (WordInterval s e) (l2br_negation_type_intersect ls)" |
-    "l2br_negation_type_intersect ((Neg (s,e))#ls) = wordinterval_intersection (wordinterval_invert (WordInterval s e)) (l2br_negation_type_intersect ls)"
-
-  lemma l2br_negation_type_intersect_alt: "wordinterval_to_set (l2br_negation_type_intersect l) = 
-                  wordinterval_to_set (wordinterval_setminus (l2br_intersect (getPos l)) (l2br (getNeg l)))"
-    apply(simp add: l2br_intersect l2br)
-    apply(induction l rule :l2br_negation_type_intersect.induct)
-       apply(simp_all)
-      apply(fast)+
-    done
-
-  lemma l2br_negation_type_intersect: "wordinterval_to_set (l2br_negation_type_intersect l) = 
-                        (\<Inter> (i,j) \<in> set (getPos l). {i .. j}) - (\<Union> (i,j) \<in> set (getNeg l). {i .. j})"
-    by(simp add: l2br_negation_type_intersect_alt l2br_intersect l2br)
-
-
   definition ipt_ipv4range_negation_type_to_br_intersect :: "ipt_ipv4range negation_type list \<Rightarrow> 32 wordinterval" where
     "ipt_ipv4range_negation_type_to_br_intersect l = l2br_negation_type_intersect (NegPos_map ipt_ipv4range_to_intervall l)" 
 
